remove some assumes

src/Config.fst
@@ -16,7 +16,7 @@ let _ : squash (US.fits_u64)
 let _ : squash (UP.fits (FStar.Int.max_int 64))
   = A.intro_fits_ptrdiff64 ()
 
-let sc_list = admit (); [
+let sc_list1 : list sc = [
     16ul; 32ul;
     64ul; 80ul; 96ul; 112ul;
     128ul; 160ul; 192ul; 224ul;
@@ -27,51 +27,52 @@ let sc_list = admit (); [
     4096ul
   ]
 
-let sc_list_f = SizeClassSelection.sc_list_f
-
-let rec init' (n:nat) (k:nat)
-  : Pure (list nat)
-  (requires True)
-  (ensures fun r ->
-    L.length r = n
-  )
-  =
-  if n = 0
-  then []
-  else k::(init' (n-1) (k+1))
-
-let init (n:nat)
-  : list nat
-  = init' n 0
-
-let test (_:unit)
-  =
-  assert (init 0 == []);
-  assert (init 1 = [0]);
-  assert (init 2 = [0; 1])
-
-module T = FStar.Tactics
-
-let sc_list_check_aux (_:unit)
-  =
-  let l1 : list nat
-    = L.map (fun (k:sc) -> U32.v k <: nat) sc_list in
-  let l2 : list nat
-    = L.map (fun k -> sc_list_f k) (init (L.length sc_list)) in
-  let r = l1 = l2 in
-  assert (r) by T.compute();
-  assert (l1 = l2)
-
-let sc_list_lemma (i:nat{i < L.length sc_list})
-  : Lemma
-  (U32.v (L.index sc_list i) == sc_list_f i)
-  = admit ()
-
 //let sc_list = [
 //    16ul; 32ul; 64ul;
 //    128ul; 256ul; 512ul;
 //    1024ul; 2048ul; 4096ul
 //  ]
+
+let sc_list_f1 : nat -> nat = SizeClassSelection.sc_list_f
+
+open MiscList
+
+let sc_list =
+  assert_norm (L.last sc_list1 = page_size);
+  last_mem_lemma sc_list1;
+  sc_list1
+
+let sc_list_f = SizeClassSelection.sc_list_f
+
+module T = FStar.Tactics
+
+let sc_list_check (_:unit)
+  : Lemma
+  (let l1 : list nat
+    = L.map (fun (k:sc) -> U32.v k <: nat) sc_list in
+  let l2 : list nat
+    = L.map (fun k -> sc_list_f k) (init (L.length sc_list)) in
+  l1 == l2)
+  =
+  let l1 : list nat
+    = L.map (fun (k:sc) -> U32.v k <: nat) sc_list in
+  let l2 : list nat
+    = L.map (fun k -> sc_list_f k) (init (L.length sc_list)) in
+  assert (l1 = l2) by T.compute ()
+
+let sc_list_lemma (i:nat{i < L.length sc_list})
+  : Lemma
+  (U32.v (L.index sc_list i) == sc_list_f i)
+  =
+  sc_list_check ();
+  map_eq_to_index_eq
+    (fun (k:sc) -> U32.v k <: nat)
+    (fun k -> sc_list_f k)
+    (sc_list)
+    (init (L.length sc_list))
+    i;
+  init_index (L.length sc_list) i
+
 
 //DO NOT EDIT, edit sc_list instead
 let nb_size_classes
