lib_misc/MiscList.fst
@@ -1,0 +1,103 @@
+module MiscList
+
+module L = FStar.List.Tot
+
+let rec last_rev_hd_lemma (#a: Type)
+  (l: list a{Cons? l})
+  : Lemma
+  (ensures (
+    L.rev_length l;
+    L.last l == L.hd (L.rev l)
+  ))
+  (decreases L.length l)
+  = match l with
+  | [] -> ()
+  | [x] -> ()
+  | x::l' ->
+      assert (Cons? l');
+      L.rev_length l';
+      assert (Cons? (L.rev l'));
+      assert (L.last l == L.last l');
+      last_rev_hd_lemma l';
+      L.rev_append [x] l';
+      assert (L.rev l == (L.rev l')@[x]);
+      assert (L.hd (L.rev l) == L.hd (L.rev l'))
+
+let last_mem_lemma (#a: eqtype)
+  (l: list a{Cons? l})
+  : Lemma
+  (L.mem (L.last l) l)
+  =
+  let x = L.last l in
+  L.rev_length l;
+  last_rev_hd_lemma l;
+  assert (x == L.hd (L.rev l));
+  assert (L.mem x (L.rev l));
+  L.rev_mem l x;
+  assert (L.mem x l)
+
+let rec init' (n:nat) (k:nat)
+  : Pure (list nat)
+  (requires True)
+  (ensures fun r ->
+    L.length r = n
+  )
+  =
+  if n = 0
+  then []
+  else k::(init' (n-1) (k+1))
+
+let init (n:nat)
+  : list nat
+  = init' n 0
+
+let rec init_index' (n:nat) (k:nat) (i:nat{i < n})
+  : Lemma
+  (L.index (init' n k) i == i + k)
+  =
+  if n = 0 || i = 0
+  then ()
+  else init_index' (n-1) (k+1) (i-1)
+
+let init_index (n: nat) (i:nat{i < n})
+  : Lemma
+  (L.index (init n) i == i)
+  = init_index' n 0 i
+
+let test (_:unit)
+  =
+  assert (init 0 == []);
+  assert (init 1 = [0]);
+  assert (init 2 = [0; 1])
+
+let rec map_index
+  (#a #b: Type)
+  (f: a -> b)
+  (l: list a)
+  (i: nat{i < L.length l})
+  : Lemma
+  (L.index (L.map f l) i == f (L.index l i))
+  = match l with
+  | [] -> ()
+  | x::tl -> if i = 0 then () else (
+      assert (L.length tl = L.length l - 1);
+      map_index f tl (i-1)
+    )
+
+let map_eq_to_index_eq
+  (#a #b #c: Type)
+  (f1: a -> c)
+  (f2: b -> c)
+  (init1: list a)
+  (init2: list b)
+  (i: nat{i < L.length init1})
+  : Lemma
+  (requires
+    L.map f1 init1 == L.map f2 init2
+  )
+  (ensures
+    f1 (L.index init1 i) == f2 (L.index init2 i)
+  )
+  =
+  map_index f1 init1 i;
+  map_index f2 init2 i
